James C - switched to debruijn. Subst lemma almost done

isabelle/AssocList.thy
@@ -55,4 +55,68 @@ by (induction env, auto)
 lemma [simp]: "lookup env k = None ==> strip_binding env k = env" 
 by (induction env, auto)
 
+primrec extend_at :: "(nat, 'b) assoc => nat => 'b => (nat, 'b) assoc" 
+where "extend_at (ASSOC env) k v = ASSOC (%kp. case kp of
+          Suc kpp => if Suc kpp < k then env kp else if Suc kpp = k then Some v else env kpp
+        | 0 => if k = 0 then Some v else env kp)"
+
+lemma [simp]: "lookup (extend_at env x v) x = Some v"
+by (induction env, cases x, simp_all)
+
+lemma [simp]: "v < n ==> lookup (extend_at env n k) v = lookup env v" 
+by (induction env, cases v, simp_all)
+
+lemma [simp]: "v >= n ==> lookup (extend_at env n k) (Suc v) = lookup env v" 
+by (induction env, cases v, simp_all)
+
+lemma extend_at_swap: "extend_at (extend_at env 0 r) (Suc n) k = extend_at (extend_at env n k) 0 r"
+proof (induction env)
+case (ASSOC f)
+  have "ALL x. (\<lambda>kp. case kp of 0 \<Rightarrow> if Suc n = 0 then Some k else case kp of 0 \<Rightarrow> if 0 = 0 then Some r else f kp | Suc kpp \<Rightarrow> if Suc kpp < 0 then f kp else if Suc kpp = 0 then Some r else f kpp
+          | Suc kpp \<Rightarrow> if Suc kpp < Suc n then case kp of 0 \<Rightarrow> if 0 = 0 then Some r else f kp | Suc kpp \<Rightarrow> if Suc kpp < 0 then f kp else if Suc kpp = 0 then Some r else f kpp
+                      else if Suc kpp = Suc n then Some k
+                           else case kpp of 0 \<Rightarrow> if 0 = 0 then Some r else f kpp | Suc kppa \<Rightarrow> if Suc kppa < 0 then f kpp else if Suc kppa = 0 then Some r else f kppa) x =
+    (\<lambda>kp. case kp of 0 \<Rightarrow> if 0 = 0 then Some r else case kp of 0 \<Rightarrow> if n = 0 then Some k else f kp | Suc kpp \<Rightarrow> if Suc kpp < n then f kp else if Suc kpp = n then Some k else f kpp
+          | Suc kpp \<Rightarrow> if Suc kpp < 0 then case kp of 0 \<Rightarrow> if n = 0 then Some k else f kp | Suc kpp \<Rightarrow> if Suc kpp < n then f kp else if Suc kpp = n then Some k else f kpp
+                      else if Suc kpp = 0 then Some r else case kpp of 0 \<Rightarrow> if n = 0 then Some k else f kpp | Suc kppa \<Rightarrow> if Suc kppa < n then f kpp else if Suc kppa = n then Some k else f kppa) x"
+  proof auto
+    fix x
+    show "(case x of 0 \<Rightarrow> case x of 0 \<Rightarrow> Some r | Suc kpp \<Rightarrow> if Suc kpp < 0 then f x else if Suc kpp = 0 then Some r else f kpp
+         | Suc kpp \<Rightarrow> if Suc kpp < Suc 0 then case x of 0 \<Rightarrow> Some r | Suc kpp \<Rightarrow> if Suc kpp < 0 then f x else if Suc kpp = 0 then Some r else f kpp
+                     else if Suc kpp = Suc 0 then Some k
+                          else case kpp of 0 \<Rightarrow> if (0\<Colon>'d) = (0\<Colon>'d) then Some r else f kpp | Suc kppa \<Rightarrow> if Suc kppa < 0 then f kpp else if Suc kppa = 0 then Some r else f kppa) =
+        (case x of 0 \<Rightarrow> Some r
+         | Suc kpp \<Rightarrow> if Suc kpp < 0 then case x of 0 \<Rightarrow> Some k | Suc kpp \<Rightarrow> if Suc kpp < 0 then f x else if Suc kpp = 0 then Some k else f kpp
+                     else if Suc kpp = 0 then Some r else case kpp of 0 \<Rightarrow> if 0 = 0 then Some k else f kpp | Suc kppa \<Rightarrow> if Suc kppa < 0 then f kpp else if Suc kppa = 0 then Some k else f kppa)"
+    proof (cases x)
+    case 0
+      thus ?thesis by simp
+    next case (Suc xx)
+      thus ?thesis by (cases xx, simp_all)
+    qed
+  next
+    fix x
+    show "(case x of 0 \<Rightarrow> case x of 0 \<Rightarrow> Some r | Suc kpp \<Rightarrow> if Suc kpp < 0 then f x else if Suc kpp = 0 then Some r else f kpp
+         | Suc kpp \<Rightarrow> if Suc kpp < Suc n then case x of 0 \<Rightarrow> Some r | Suc kpp \<Rightarrow> if Suc kpp < 0 then f x else if Suc kpp = 0 then Some r else f kpp
+                     else if Suc kpp = Suc n then Some k
+                          else case kpp of 0 \<Rightarrow> if (0\<Colon>'d) = (0\<Colon>'d) then Some r else f kpp | Suc kppa \<Rightarrow> if Suc kppa < 0 then f kpp else if Suc kppa = 0 then Some r else f kppa) =
+        (case x of 0 \<Rightarrow> Some r
+         | Suc kpp \<Rightarrow> if Suc kpp < 0 then case x of 0 \<Rightarrow> f x | Suc kpp \<Rightarrow> if Suc kpp < n then f x else if Suc kpp = n then Some k else f kpp
+                     else if Suc kpp = 0 then Some r else case kpp of 0 \<Rightarrow> if n = 0 then Some k else f kpp | Suc kppa \<Rightarrow> if Suc kppa < n then f kpp else if Suc kppa = n then Some k else f kppa)"
+    proof (cases x)
+    case 0
+      thus ?thesis by simp
+    next case (Suc xx)
+      thus ?thesis by (cases xx, simp_all)
+    qed
+  qed
+  thus ?case by auto
+qed
+
+lemma [simp]: "extend_at (extend env x k) 0 r = extend (extend_at env 0 r) (Suc x) k"
+proof (induction env)
+case (ASSOC f)
+  thus ?case sorry
+qed
+
 end
